### 3:
  - 0 -> 2 ...
### 4:
  - 0 -> 3 -> 4 ...
### 5:
  - 0 -> 4 -> 6 ...
### 6:
  - 0 -> 5 -> 8 -> 9 ... 
### 7:
  - 0 -> 6 -> 10 -> 12 ...
### 8:
  - 0 -> 7 -> 12 -> 15 -> 16 ...

x * (t - x) > d
-x^2 + tx - d > 0

# x(-x + t) - d > 0
# x = (-t +- sqrt(t^2 - 4d)) / -2:
  - x > (-t + sqrt(t^2 - 4d)) / -2:
  - x < (-t - sqrt(t^2 - 4d)) / -2:

```
t = 30, d = 200

x > (-30 + sqrt(900 - 800)) / -2
x > (-30 + 10) / -2
x > 10 -> 11

x < (-30 - sqrt(900 - 800)) / -2
x < (-30 - 10) / 02
x < 20 -> 19

19 - 11 + 1 = 9
```
